WIP WP definition over Pred

theories/stlc/Symbolic.v
@@ -1358,5 +1358,29 @@ Section Correctness.
       apply RQ; auto. f_equal. clear.
       admit.
   Admitted.
+  Print WP.
 
 End Correctness.
+
+
+Section WithPredicates.
+
+  Import Pred Pred.notations.
+
+  Definition WP {A} : ⊢ FreeM A -> □⁺(A -> Pred) -> Pred.
+  refine (
+    fix WP (w : World) (m : FreeM A w) (POST : □⁺(A -> Pred) w) {struct m} :=
+      match m with
+      | Ret_Free _ _ v => T POST v
+      | Fail_Free _ _ => ⊥ₚ%P
+      | Bind_AssertEq_Free _ _ t1 t2 k => (t1 =ₚ t2 /\ₚ WP w k POST)%P
+      | Bind_Exists_Free _ _ i k => (∃ₚ t ∶ Ty, Ext _ (@thick _ _ _ i ctx.in_zero t))%P
+      end).
+  Proof. admit.
+     apply WP. apply k. Print Alloc. Check alloc.fresh w i _ _. apply (_4 POST (alloc.fresh w i _ refl)).
+     admit.
+     Unshelve. admit.
+  Admitted.
+
+
+End WithPredicates.
